src/Analysis/Instances/Parity/Ctx/Parity_Ctx_None_Sound.thy
@@ -5,6 +5,7 @@ theory Parity_Ctx_None_Sound
     "Voblint_Core.DG_Base"
     "Voblint_Exec.DG_Base_Exec"
     "Voblint_Analysis.Parity_Exec"
+    "Voblint_Analysis.Parity_Sound"
     "Voblint_Compile.Compile_Invariants"
     "Voblint_CFG.CFG_Prune"
     "TD.TD_side_upd_rule"
@@ -49,17 +50,6 @@ text \<open>
   spec, and every domain-transfer soundness fact about the spec is untouched by
   that wrapping.
 \<close>
-
-definition pctx_spec ::
-  "(vname \<Rightarrow> bool) \<Rightarrow> (parity exec_dg_st \<Rightarrow> bool)
-     \<Rightarrow> ('x, 'k, unit, parity exec_dg_st lifted, parity exec_dg_st lifted) dg_spec"
-where
-  "pctx_spec gs empty_pred =
-     base_dg_spec_st_for_lifted gs empty_pred (parity_tf_st_for gs) (parity_enter_st_for gs)"
-
-definition pctx_abs_spec ::
-    "(vname \<Rightarrow> bool) \<Rightarrow> ('x, 'k, unit, parity abs_state lifted, parity abs_state lifted) dg_spec" where
-  "pctx_abs_spec gs = base_dg_spec_for_lifted gs is_empty_state (parity_tf_for gs)"
 
 subsection \<open>The routed equation system and its executable solution\<close>
 
@@ -172,13 +162,6 @@ text \<open>
   concretization outside the interpretation so a downstream theory can state it.
 \<close>
 
-definition pctx_gamma ::
-    "(vname \<Rightarrow> bool) \<Rightarrow> parity exec_dg_st lifted \<Rightarrow> parity exec_dg_st lifted \<Rightarrow> store set" where
-  "pctx_gamma gs d g = gamma_state_lift (map_lift (fun_of_resolved_st_q_for gs) d)"
-
-lemma pctx_gamma_Bot [simp]: "pctx_gamma gs Bot g = {}"
-  by (simp add: pctx_gamma_def)
-
 definition pctx_sg_st ::
     "(vname \<Rightarrow> bool) \<Rightarrow> (parity exec_dg_st \<Rightarrow> bool) \<Rightarrow> proc_table \<Rightarrow> pname list
        \<Rightarrow> pp \<times> unit + gk \<Rightarrow> parity exec_dg_st lifted" where
@@ -201,13 +184,6 @@ interpretation parity_unit: routed_domain_exec
   by unfold_locales
      (rule parity_tf_st_for_commute, rule parity_enter_st_for_commute, rule exact, simp, simp,
       simp add: static_resolve_def)
-
-lemma pctx_gamma_eq: "pctx_gamma gs = parity_unit.gamma_exec"
-  by (intro ext) (simp add: pctx_gamma_def parity_unit.gamma_exec_def gamma_dg_base_def)
-
-theorem pctx_sound_exec: "sound_dg_spec (pctx_spec gs empty_pred) (pctx_gamma gs) gs"
-  unfolding pctx_gamma_eq pctx_spec_def
-  by (rule parity_unit.sound_dg_spec_st[OF parity_is_sound_transfer_for])
 
 end
 
